\input{preamble.sty}

\begin{document}

\section{$y' + 2y = e^{-x}$}

\begin{align*}
    y' & = e^{-x} - 2y                                                \\
    y  & = \left( C + \int e^{-x}e^{\int 2dx} dx \right)e^{-\int 2dx} \\
    y  & = \left( C + e^{C_1}\int e^{x} dx \right)e^{-2x}e^{-C_1}     \\
    y  & = \left( C +  e^{C_1}e^x \right)e^{-2x} e^{-C_1}             \\
    y  & = \left( Ce^{-C_1}e^{-2x} +  e^{-x} \right)                  \\
    y  & = \left( Ce^{-2x} +  e^{-x} \right)                          \\
\end{align*}

\section{$y'-y\tg x=\cfrac{1}{\cos^3x}, y(0)=0$}

\begin{align*}
    y'   & = y\tg x + \frac{1}{\cos^3x}                                                                                                          \\
    p(x) & = \tg x \quad q(x) = \frac{1}{\cos^3 x}                                                                                               \\
    y    & = \left( C + \int \frac{1}{\cos^3 x} e^{-\int \tg x dx} dx \right)e^{-\int \tg x dx}                                                  \\
    y    & = \left( C + \int \frac{1}{\cos^3 x} e^{-\ln \cos x - C_1} dx \right)e^{\ln \cos x + C_1}                                             \\
    y    & = \left( C + \int \frac{1}{\cos^3 x} \cos^{-1} x e^{-C_1} dx \right)\cos x e^{C_1}                                                    \\
    y    & = \left( C + e^{-C_1} \int \frac{1}{\cos^4 x} dx \right)\cos x e^{C_1}                                                                \\
    y    & = \left( C + e^{-C_1} \left(\frac{1}{3}\frac{\tg x}{\cos^2 x} + \frac{2}{3} \int \frac{1}{\cos^2 x}dx\right) dx \right)\cos x e^{C_1} \\
    y    & = \left( C + e^{-C_1} \left(\frac{1}{3}\frac{\tg x}{\cos^2 x} + \frac{2}{3} \tg x \right)\right)\cos x e^{C_1}                        \\
    y    & = \left( C \cos x + e^{-C_1} \left(\frac{1}{3}\frac{\tg x}{\cos x} + \frac{2}{3} \sin x \right)\right) e^{C_1}                        \\
    y    & = e^{C_1}C \cos x + \left(\frac{1}{3}\frac{\tg x}{\cos x} + \frac{2}{3} \sin x \right)                                                \\
    0    & = e^{C_1}C + 0                                                                                                                        \\
    C    & = 0                                                                                                                                   \\
    y    & = \left(\frac{1}{3}\frac{\tg x}{\cos x} + \frac{2}{3} \sin x \right)                                                                  \\
\end{align*}

\section{$y'-y\ln 2=2^{\sin x}(\cos x - 1)\ln 2$, y ограничено при $\to\infty$}

\begin{align*}
    y' & = y\ln 2 + 2^{\sin x}(\cos x - 1)\ln 2                                \\
    y  & \xrightarrow[x\to \infty]{} \frac{y'}{\ln 2} - 2^{\sin x}(\cos x - 1)
\end{align*}

\section*{$y'-y\cos x = y^2 \cos x$}

\begin{align*}
    y' & = y\cos x(y+1)
\end{align*}

$y \equiv 0$ подходит, $y\equiv -1$ тоже подходит.

$\sphericalangle y\not\in\{0, -1\}$

\begin{align*}
    \frac{dy}{dx}\frac{1}{y(y+1)}           & = \cos x        \\
    \frac{dy}{y(y+1)}                       & = dx\cos x      \\
    \int \frac{dy}{y(y+1)}                  & = \int dx\cos x \\
    \int \frac{dy}{y(y+1)}                  & = \sin x + C    \\
    \int \frac{dy}{y(y+1)}                  & = \sin x + C    \\
    \int \frac{dy}{y} - \int \frac{dy}{y+1} & = \sin x + C    \\
    \ln |y| - \ln|y+1|                      & = \sin x + C    \\
\end{align*}

\end{document}